Added sum types.

src/Stlc.v
@@ -7,12 +7,14 @@ Inductive ty : Type :=
   | TArrow : ty -> ty -> ty         (* T -> T *)
   | TBool  : ty                     (* Bool *)
   | TUnit  : ty                     (* Unit *)
-  | TProd  : ty -> ty -> ty.        (* (T1, T2) *)
+  | TProd  : ty -> ty -> ty         (* T1 * T2 *)
+  | TSum   : ty -> ty -> ty         (* T1 + T2 *)
+  .
 
 Tactic Notation "T_cases" tactic(first) ident(c) :=
   first;
   [ Case_aux c "TArrow" | Case_aux c "TBool"
-  | Case_aux c "TUnit" | Case_aux c "TProd" ].
+  | Case_aux c "TUnit" | Case_aux c "TProd" | Case_aux c "TSum" ].
 
 Inductive tm : Type :=
   | tvar : id -> tm                 (* x *)
@@ -25,6 +27,9 @@ Inductive tm : Type :=
   | tpair : tm -> tm -> tm          (* (t1, t2) *)
   | tfst : tm -> tm                 (* fst t1 *)
   | tsnd : tm -> tm                 (* snd t1 *)
+  | tinl : ty -> tm -> tm           (* inl T t *)
+  | tinr : ty -> tm -> tm           (* inr T t *)
+  | tcase : tm -> tm -> tm -> tm    (* case t0 t1 t2 *)
   .
 
 Tactic Notation "t_cases" tactic(first) ident(c) :=
@@ -32,7 +37,8 @@ Tactic Notation "t_cases" tactic(first) ident(c) :=
   [ Case_aux c "tvar" | Case_aux c "tapp" 
   | Case_aux c "tabs" | Case_aux c "ttrue" 
   | Case_aux c "tfalse" | Case_aux c "tif" | Case_aux c "tunit" 
-  | Case_aux c "tpair" | Case_aux c "tfst" | Case_aux c "tsnd" ].
+  | Case_aux c "tpair" | Case_aux c "tfst" | Case_aux c "tsnd" 
+  | Case_aux c "tinl" | Case_aux c "tinr" | Case_aux c "tcase" ].
 
 Definition x := (Id 0).
 Definition y := (Id 1).
@@ -52,13 +58,18 @@ Inductive value : tm -> Prop :=
       value tunit 
   | v_pair : forall t1 t2,
       value (tpair t1 t2)
+  | v_inl : forall T t,
+      value (tinl T t)
+  | v_inr : forall T t,
+      value (tinr T t)
   .
 
 Tactic Notation "v_cases" tactic(first) ident(c) :=
   first;
   [ Case_aux c "v_abs" | Case_aux c "v_true"
   | Case_aux c "v_false" | Case_aux c "v_unit"
-  | Case_aux c "v_pair" ].
+  | Case_aux c "v_pair"
+  | Case_aux c "v_inl" | Case_aux c "v_inr" ].
 
 Hint Constructors value.
 
@@ -86,6 +97,12 @@ Fixpoint subst (x:id) (s:tm) (t:tm) : tm :=
       tfst ([x:=s] t1)
   | tsnd t1 =>
       tsnd ([x:=s] t1)
+  | tinl T t1 =>
+      tinl T ([x:=s] t1)
+  | tinr T t1 =>
+      tinr T ([x:=s] t1)
+  | tcase t1 t2 t3 =>
+      tcase ([x:=s] t1) ([x:=s] t2) ([x:=s] t3)
   end
 
 where "'[' x ':=' s ']' t" := (subst x s t).
@@ -116,6 +133,13 @@ Inductive step : tm -> tm -> Prop :=
   | ST_Snd : forall t t',
       t ==> t' ->
       tsnd t ==> tsnd t'
+  | ST_CaseInl : forall T t1 t2 t3,
+      (tcase (tinl T t1) t2 t3) ==> (tapp t2 t1)
+  | ST_CaseInr : forall T t1 t2 t3,
+      (tcase (tinr T t1) t2 t3) ==> (tapp t3 t1)
+  | ST_Case : forall t1 t1' t2 t3,
+      t1 ==> t1' ->
+      tcase t1 t2 t3 ==> tcase t1' t2 t3
 
 where "t1 '==>' t2" := (step t1 t2).
 
@@ -124,7 +148,8 @@ Tactic Notation "step_cases" tactic(first) ident(c) :=
   [ Case_aux c "ST_AppAbs" | Case_aux c "ST_App1" 
   | Case_aux c "ST_IfTrue" | Case_aux c "ST_IfFalse" | Case_aux c "ST_If"
   | Case_aux c "ST_FstPair" | Case_aux c "ST_Fst"
-  | Case_aux c "ST_SndPair" | Case_aux c "St_Snd"].
+  | Case_aux c "ST_SndPair" | Case_aux c "ST_Snd"
+  | Case_aux c "ST_CaeInl" | Case_aux c "ST_CaseInr" | Case_aux c "ST_Case" ].
 
 Hint Constructors step.
 
@@ -167,6 +192,17 @@ Inductive has_type : context -> tm -> ty -> Prop :=
   | T_Snd : forall Gamma t T1 T2,
        Gamma |- t \in (TProd T1 T2) ->
        Gamma |- (tsnd t) \in T2
+  | T_Inl : forall Gamma t T1 T2,
+       Gamma |- t \in T1 ->
+       Gamma |- (tinl T2 t) \in (TSum T1 T2)
+  | T_Inr : forall Gamma t T1 T2,
+       Gamma |- t \in T2 ->
+       Gamma |- (tinr T1 t) \in (TSum T1 T2)
+  | T_Case : forall Gamma t1 t2 t3 T1 T2 T3,
+       Gamma |- t1 \in (TSum T1 T2) ->
+       Gamma |- t2 \in (TArrow T1 T3) ->
+       Gamma |- t3 \in (TArrow T2 T3) ->
+       Gamma |- (tcase t1 t2 t3) \in T3
 
 where "Gamma '|-' t '\in' T" := (has_type Gamma t T).
 
@@ -176,7 +212,8 @@ Tactic Notation "has_type_cases" tactic(first) ident(c) :=
   | Case_aux c "T_App" | Case_aux c "T_True" 
   | Case_aux c "T_False" | Case_aux c "T_If" 
   | Case_aux c "T_Unit" 
-  | Case_aux c "T_Pair" | Case_aux c "T_Fst" | Case_aux c "T_Snd" ].
+  | Case_aux c "T_Pair" | Case_aux c "T_Fst" | Case_aux c "T_Snd" 
+  | Case_aux c "T_Inl" | Case_aux c "T_Inr" | Case_aux c "T_Case" ].
 
 Hint Constructors has_type.
 
